Stopped at the unfold/reify smt-encoding problem

examples/rel/IfcReify.fst
@@ -7,129 +7,129 @@ open FStar.DM4F.IntStore
 open FStar.Classical
 
 (* Just for debug *)
-let ni_exp (e:exp)  = forall (h: heap). b2t (normalize_term (fst (interpret_exp h e)) = Some 5)
+(* let ni_exp (e:exp)  = forall (h: heap). b2t (normalize_term (fst (interpret_exp h e)) = Some 5) *)
 
-(* (\****************************** Preliminaries ******************************\) *)
+(****************************** Preliminaries ******************************)
 
-(* (\* CH: Everything specialized to 2-point lattice *\) *)
-(* type label = *)
-(* | Low *)
-(* | High *)
+(* CH: Everything specialized to 2-point lattice *)
+type label =
+| Low
+| High
 
-(* val op_Less : label -> label -> Tot bool *)
-(* let op_Less l1 l2 = *)
-(*   match l1, l2 with *)
-(*   | Low,High -> true *)
-(*   | _, _ -> false *)
+val op_Less : label -> label -> Tot bool
+let op_Less l1 l2 =
+  match l1, l2 with
+  | Low,High -> true
+  | _, _ -> false
 
-(* val op_Less_Equals : label -> label -> Tot bool *)
-(* let op_Less_Equals l1 l2 = *)
-(*   match l1, l2 with *)
-(*   | High,Low -> false *)
-(*   | _, _ -> true *)
+val op_Less_Equals : label -> label -> Tot bool
+let op_Less_Equals l1 l2 =
+  match l1, l2 with
+  | High,Low -> false
+  | _, _ -> true
 
-(* val join : label -> label -> Tot label *)
-(* let join l1 l2 = *)
-(*   match l1, l2 with *)
-(*   | Low,Low -> Low *)
-(*   | _, _ -> High *)
+val join : label -> label -> Tot label
+let join l1 l2 =
+  match l1, l2 with
+  | Low,Low -> Low
+  | _, _ -> High
 
-(* type label_fun = nat -> Tot label *)
+type label_fun = nat -> Tot label
 
-(* let in_r x h = (in_ x) `diagb` h *)
+let in_r x h = (in_ x) `diagb` h
 
-(* type low_equiv (env:label_fun) (h1:rel heap) = *)
-(*   forall (x:id{x `in_r` h1}). *)
-(*     env x = Low ==> index (R?.l h1) x = index (R?.r h1) x *)
+type low_equiv (env:label_fun) (h1:rel heap) =
+  forall (x:id{x `in_r` h1}).
+    env x = Low ==> index (R?.l h1) x = index (R?.r h1) x
 
-(* let get_heap (#a:Type) : option a * heap -> Tot (option heap) *)
-(* = function *)
-(*   | None, _ -> None *)
-(*   | Some _, h -> Some h *)
+let get_heap (#a:Type) : option a * heap -> Tot (option heap)
+= function
+  | None, _ -> None
+  | Some _, h -> Some h
 
-(* (\**************************** Typing Judgements ****************************\) *)
+(**************************** Typing Judgements ****************************)
 
-(* (\* env |- e : l *)
-(*    - Expressions do not modify the heap *)
-(*    - Correctness *)
-(*    - Low equivalent input heaps + Low label ==> same result *)
-(* *\) *)
+(* env |- e : l
+   - Expressions do not modify the heap
+   - Correctness
+   - Low equivalent input heaps + Low label ==> same result
+*)
+unfold
+let ni_exp (env:label_fun) (e:exp) (l:label) : Tot Type0 =
+  forall (h: rel heap).
+   (low_equiv env h /\ Low? l) ==>
+     b2t (normalize_term (fst (interpret_exp (R?.r h) e)) = normalize_term (fst (interpret_exp (R?.l h) e)))
+
+(* env,pc:l |- c
+   - References with a label below l are not modified
+   - Total correctness
+   - Low equivalent input heaps ==> Low equivalent output heaps
+*)
+let inv_com' (env:label_fun) (c:com) (l:label) (h0_opt:option heap) : Tot Type0
+= match h0_opt with
+  | None -> True
+  | Some h0 ->
+    match interpret_com h0 c with
+    | None -> True
+    | Some h1 ->
+      forall (i:id{i `in_` h0 }). env i < l ==> index h0 i = index h1 i
+
+let ni_com' (env:label_fun) (c:com) (l:label) (h0_opt: rel (option heap)) =
+  match h0_opt with
+  | R (Some h0l) (Some h0r) ->
+    (* KM : That's the code that we would like to write but subtyping and matching on pairs interplay badly *)
+    (* it generates a VC which boils down to [forall (h1l:heap). length h1l = length h0l] which is obviously false *)
+    (* begin match interpret_com h0l c, interpret_com h0r c with *)
+    (* | Some h1l, Some h1r -> low_equiv env (R h0l h0r) ==> low_equiv env (R h1l h1r) *)
+    (* | _ -> True *)
+    (* end *)
+    begin match interpret_com h0l c with
+      | Some h1l -> begin match  interpret_com h0r c with
+        | Some h1r -> low_equiv env (R h0l h0r) ==> low_equiv env (R h1l h1r)
+        | _ -> True
+      end
+      | _ -> True
+    end
+  | _ -> True
+
+let ni_com (env:label_fun) (c:com) (l:label) =
+  (forall (h0: rel (option heap)). ni_com' env c l h0) /\
+  (forall (h0:option heap). inv_com' env c l h0)
+
+(* KM : Trying to figure out wht are the design tradeoffs on option heap *)
 (* unfold *)
-(* let ni_exp (env:label_fun) (e:exp) (l:label) = *)
-(*   forall (h: rel heap). *)
-(*    (low_equiv env h /\ Low? l) ==> *)
-(*      b2t (normalize_term (fst (interpret_exp (R?.r h) e)) = normalize_term (fst (interpret_exp (R?.l h) e))) *)
+(* let preserves_env_upto_label (env:label_fun) (l:label) (c:com) (h0:heap) : Tot Type0 *)
+(* = let (res, h1) = interpret_com h0 c in *)
+(*   Some? res ==> (forall (i:id{i `in_` h0}). env i < l ==> index h0 i = index h1 i) *)
 
-(* (\* env,pc:l |- c *)
-(*    - References with a label below l are not modified *)
-(*    - Total correctness *)
-(*    - Low equivalent input heaps ==> Low equivalent output heaps *)
-(* *\) *)
-(* let inv_com' (env:label_fun) (c:com) (l:label) (h0_opt:option heap) : Tot Type0 *)
-(* = match h0_opt with *)
-(*   | None -> True *)
-(*   | Some h0 -> *)
-(*     match interpret_com h0 c with *)
-(*     | None -> True *)
-(*     | Some h1 -> *)
-(*       forall (i:id{i `in_` h0 }). env i < l ==> index h0 i = index h1 i *)
+(* type ni_com' (env:label_fun) (c:com) (l:label) (h0:rel heap) = *)
+(*   begin *)
+(*     let res, h1 = split (lift (fun h -> interpret_com h c) h0) in *)
+(*     low_equiv env h0 /\ Some? `diagb` res ==> low_equiv env h1 *)
+(*     end /\ *)
+(*     (preserves_env_upto_label env l c) `diag` h0 *)
 
-(* let ni_com' (env:label_fun) (c:com) (l:label) (h0_opt: rel (option heap)) = *)
-(*   match h0_opt with *)
-(*   | R (Some h0l) (Some h0r) -> *)
-(*     (\* KM : That's the code that we would like to write but subtyping and matching on pairs interplay badly *\) *)
-(*     (\* it generates a VC which boils down to [forall (h1l:heap). length h1l = length h0l] which is obviously false *\) *)
-(*     (\* begin match interpret_com h0l c, interpret_com h0r c with *\) *)
-(*     (\* | Some h1l, Some h1r -> low_equiv env (R h0l h0r) ==> low_equiv env (R h1l h1r) *\) *)
-(*     (\* | _ -> True *\) *)
-(*     (\* end *\) *)
-(*     begin match interpret_com h0l c with *)
-(*       | Some h1l -> begin match  interpret_com h0r c with *)
-(*         | Some h1r -> low_equiv env (R h0l h0r) ==> low_equiv env (R h1l h1r) *)
-(*         | _ -> True *)
-(*       end *)
-(*       | _ -> True *)
-(*     end *)
-(*   | _ -> True *)
+(* type ni_com (env:label_fun) (c:com) (l:label) = *)
+(*     forall (h0: rel heap). ni_com' env c l h0 *)
 
-(* let ni_com (env:label_fun) (c:com) (l:label) = *)
-(*   (forall (h0: rel (option heap)). ni_com' env c l h0) /\ *)
-(*   (forall (h0:option heap). inv_com' env c l h0) *)
+(*********************** Typing Rules for Expressions **********************)
 
-(* (\* KM : Trying to figure out wht are the design tradeoffs on option heap *\) *)
-(* (\* unfold *\) *)
-(* (\* let preserves_env_upto_label (env:label_fun) (l:label) (c:com) (h0:heap) : Tot Type0 *\) *)
-(* (\* = let (res, h1) = interpret_com h0 c in *\) *)
-(* (\*   Some? res ==> (forall (i:id{i `in_` h0}). env i < l ==> index h0 i = index h1 i) *\) *)
+(* CH: The way we derive these rules looks more like a
+       semantically-justified program logic than a syntactic type
+       system. Any connection to Dave Naumann and Anindya Banerjee's
+       "relational logic"? (e.g. https://arxiv.org/abs/1611.08992) *)
 
-(* (\* type ni_com' (env:label_fun) (c:com) (l:label) (h0:rel heap) = *\) *)
-(* (\*   begin *\) *)
-(* (\*     let res, h1 = split (lift (fun h -> interpret_com h c) h0) in *\) *)
-(* (\*     low_equiv env h0 /\ Some? `diagb` res ==> low_equiv env h1 *\) *)
-(* (\*     end /\ *\) *)
-(* (\*     (preserves_env_upto_label env l c) `diag` h0 *\) *)
+(* Subtyping rule for expression labels
 
-(* (\* type ni_com (env:label_fun) (c:com) (l:label) = *\) *)
-(* (\*     forall (h0: rel heap). ni_com' env c l h0 *\) *)
+         E |- e : l1   l1 <= l2
+         ----------------------
+              E |- e : l2
+*)
 
-(* (\*********************** Typing Rules for Expressions **********************\) *)
-
-(* (\* CH: The way we derive these rules looks more like a *)
-(*        semantically-justified program logic than a syntactic type *)
-(*        system. Any connection to Dave Naumann and Anindya Banerjee's *)
-(*        "relational logic"? (e.g. https://arxiv.org/abs/1611.08992) *\) *)
-
-(* (\* Subtyping rule for expression labels *)
-
-(*          E |- e : l1   l1 <= l2 *)
-(*          ---------------------- *)
-(*               E |- e : l2 *)
-(* *\) *)
-
-(* val sub_exp : env:label_fun -> e:exp -> l1:label -> l2:label{l1 <= l2} -> *)
-(*   Lemma (requires (ni_exp env e l1)) *)
-(*         (ensures  (ni_exp env e l2)) *)
-(* let sub_exp _ _ _ _ = () *)
+val sub_exp : env:label_fun -> e:exp -> l1:label -> l2:label{l1 <= l2} ->
+  Lemma (requires (ni_exp env e l1))
+        (ensures  (ni_exp env e l2))
+let sub_exp _ _ _ _ = ()
 
 
 
